project/inductive/basic/inductive_graph_basic.v
@@ -54,36 +54,36 @@ Compute isEmpty empty.
 (* Here start the helper functions for "matsh" *)
 
 (* Applies a function to a map entry if it exists quickly *)
-Definition updateEntry (n : Node) (f : (NatSet.t * NatSet.t) -> (NatSet.t * NatSet.t)) (ig : IG) : IG :=
-  match NatMap.find n ig with
-    | Some v => NatMap.add n (f v) ig
+Definition updateEntry (node : Node) (f : (NatSet.t * NatSet.t) -> (NatSet.t * NatSet.t)) (ig : IG) : IG :=
+  match NatMap.find node ig with
+    | Some v => NatMap.add node (f v) ig
     | None => ig
   end.
 
 
-Definition cleanUp' (n : Node) (froms tos : NatSet.t) (ig : IG) : IG :=
+Definition cleanUp' (node : Node) (froms tos : NatSet.t) (ig : IG) : IG :=
   (* Loop over ingoing edges of removed node to update the outgoing of all of those to not have n anymore *)
   let ig' := NatSet.fold (fun (elem : Node) (acc : IG) =>
-  updateEntry elem (fun '(currFroms, currTos) => (NatSet.remove n currFroms, currTos))
+  updateEntry elem (fun '(currFroms, currTos) => (NatSet.remove node currFroms, currTos))
     acc) tos ig in
 
   (* Loop over outgoing edges of removed node to update the ingoing of all of those to not have n anymore *)
   NatSet.fold (fun (elem : Node) (acc : IG) =>
-  updateEntry elem (fun '(currFroms, currTos) => (currFroms, NatSet.remove n currTos))
+  updateEntry elem (fun '(currFroms, currTos) => (currFroms, NatSet.remove node currTos))
     acc) froms ig'.
   
 
 
-Definition cleanUp(n : Node) (context : (NatSet.t * NatSet.t)) (ig : IG) : IG :=
+Definition cleanUp (node : Node) (context : (NatSet.t * NatSet.t)) (ig : IG) : IG :=
   match context with | (froms, tos) =>
-    cleanUp' n froms tos (NatMap.remove n ig)
+    cleanUp' node froms tos (NatMap.remove node ig)
   end.
 
 
-Definition matsh (n : Node) (ig : IG) : (option (NatSet.t * NatSet.t) * IG) :=
-  match NatMap.find n ig with
+Definition matsh (node : Node) (ig : IG) : (option (NatSet.t * NatSet.t) * IG) :=
+  match NatMap.find node ig with
     | None => (None, ig)
-    | Some context as sContext => (sContext, cleanUp n context ig) 
+    | Some context as sContext => (sContext, cleanUp node context ig) 
   end.
 
 
@@ -91,13 +91,13 @@ Definition matsh (n : Node) (ig : IG) : (option (NatSet.t * NatSet.t) * IG) :=
 (* Here start the helper functions for "mkGraph" *)
 
 (* This is the "&" constructor, but it has to be defined as a function, since it is too advanced *)
-Definition add (n : Node) (fromsTos : (NatSet.t * NatSet.t)) (ig : IG) : IG :=
-  NatMap.add n fromsTos ig.
+Definition add (node : Node) (fromsTos : (NatSet.t * NatSet.t)) (ig : IG) : IG :=
+  NatMap.add node fromsTos ig.
 
 
 
-Definition insNode (n : Node) (ig : IG) : IG :=
-  add n (NatSet.empty, NatSet.empty) ig.
+Definition insNode (node : Node) (ig : IG) : IG :=
+  add node (NatSet.empty, NatSet.empty) ig.
   
 
 Definition insNodes (nodes : list Node) (ig : IG) : IG :=
@@ -133,6 +133,8 @@ Definition labNodes (ig : IG) : list Node :=
 
 
 
+(* Make IG_basic visible *)
+
 Definition showIG (ig : IG) :=
   map (fun '(node, (froms, tos)) => (node, (NatSet.elements froms, NatSet.elements tos))) (NatMap.elements ig).
   
@@ -144,6 +146,9 @@ Definition showDecomp (decomp : (option (NatSet.t * NatSet.t) * IG)) :=
 
 
 
+
+
+(* TODO: this should relocate to "examples" after big rename *)
 Compute showIG (mkGraph [1; 2; 3] [(1, 2); (2, 3); (3, 1)]).
 
 Definition myBasicGraph := mkGraph [1; 2; 3] [(1, 2); (2, 3); (3, 1)].
@@ -161,250 +166,3 @@ Compute showIG (mkGraph [1; 2; 3] [(1, 2); (2, 3); (3, 1)]).
 
 Compute labNodes myBasicGraph.
 
-
-
-
-(* Here, I try out various equational specifications of an IG: *)
-
-(* Block to derive useful conversion theorem "In_labNodes_is_InMap" *)
-
-(* This is from software foundations. Eventually, I will move this somewhere else *)
-Lemma eqb_reflect : forall x y, reflect (x = y) (x =? y).
-Proof.
-  intros x y. apply iff_reflect. symmetry.
-  apply Nat.eqb_eq.
-Qed.
-Lemma ltb_reflect : forall x y, reflect (x < y) (x <? y).
-Proof.
-  intros x y. apply iff_reflect. symmetry.
-  apply Nat.ltb_lt.
-Qed.
-Lemma leb_reflect : forall x y, reflect (x <= y) (x <=? y).
-Proof.
-  intros x y. apply iff_reflect. symmetry.
-  apply Nat.leb_le.
-Qed.
-
-Hint Resolve ltb_reflect leb_reflect eqb_reflect : bdestruct.
-Ltac bdestruct X :=
-  let H := fresh in let e := fresh "e" in
-   evar (e: Prop);
-   assert (H: reflect e X); subst e;
-    [ auto with bdestruct
-    | destruct H as [H|H];
-       [ | try first [apply not_lt in H | apply not_le in H]]].
-(* End from Software foundations *)
-
-Require Import Coq.micromega.Lia.
-
-Check InA.
-
-(* Helper lemma for converting an In (of a map) to an InA, which will eventually be turned to a NatMap.In (which has useful lemmas)  *)
-Lemma In_map_fst_InA : forall (A B: Type) (a : A) (l : list (A * B)),
-  In a (map fst l) <-> exists (a0 : B), InA (fun (x el : (A * B)) => x = el) (a, a0) l.
-Proof.
-  intros. induction l; simpl.
-  - split; intros.
-    + destruct H.
-    + destruct H. inversion H.
-  - split; intros.
-    + destruct H.
-      -- exists (snd a0). left. destruct a0. destruct H. simpl. reflexivity.
-      -- edestruct IHl. apply H0 in H. destruct H. exists x. apply InA_cons. right. assumption.
-    + destruct H. inversion H.
-      -- left. destruct a0. destruct H1. simpl. reflexivity.
-      -- right. apply IHl. exists x. assumption.
-Qed.  
-
-Require Import Coq.Logic.FunctionalExtensionality.
-Require Import Coq.Logic.PropExtensionality.
-
-(* Conversion from key equality from map to my own (simply written in a slightly different manner) *)
-Lemma In_conditions_same : (NatMap.eq_key_elt (elt:=NatSet.t * NatSet.t)) = (fun x el : Node * (NatSet.t * NatSet.t) => x = el).
-Proof.
-  unfold NatMap.eq_key_elt. unfold NatMap.Raw.PX.eqke.
-  apply functional_extensionality.
-  intros.
-  apply functional_extensionality.
-  intros.
-  destruct x, x0.
-  simpl.
-  apply propositional_extensionality.
-  split; intros.
-  - destruct H. subst. reflexivity.
-  - inversion H. auto.
-Qed.
-
-(* This is the most useful one for proving other statements.
-  Use it to convert from "use friendly" In- statements to "provable" NatMap.In- statements  *)
-Lemma In_labNodes_is_InMap : forall (x : Node) (ig : IG),
-  In x (labNodes ig) <-> NatMap.In x ig.
-Proof.
-  intros. unfold labNodes.
-  rewrite In_map_fst_InA.
-  pose proof (WF.elements_in_iff ig).
-  rewrite In_conditions_same in H.
-  specialize H with x.
-  symmetry.
-  assumption.
-Qed.
-
-
-(* Here start "meaningful statements" *)
-
-
-(* 5 statements on inserting (helpers for mkGraph): update, insEdge, insEdges, insNode, insNodes *)
-Lemma updateEntry_does_not_change_key_set : forall (n : Node) (f : NatSet.t * NatSet.t -> NatSet.t * NatSet.t) (ig : IG) (x : Node),
-  In x (labNodes (updateEntry n f ig)) <-> In x (labNodes ig).
-Proof.
-  intros. unfold updateEntry.
-  destruct (NatMap.find (elt:=NatSet.t * NatSet.t) n ig) eqn:isIn.
-  - rewrite In_labNodes_is_InMap. rewrite In_labNodes_is_InMap. rewrite WF.add_in_iff.
-    rewrite WF.in_find_iff. split.
-    + intros. destruct H.
-      -- rewrite <- H. rewrite isIn. unfold not. intros. discriminate H0.
-      -- assumption.
-    + intros. right. assumption.
-  - reflexivity.
-Qed.
-
-
-Lemma insEdge_does_not_add_node : forall (edge : (Node * Node)) (ig : IG) (x : Node),
-  In x (labNodes (insEdge edge ig)) <-> In x (labNodes ig).
-Proof.
-  intros. unfold insEdge. destruct edge.
-  destruct (NatMap.mem (elt:=NatSet.t * NatSet.t) n ig && NatMap.mem (elt:=NatSet.t * NatSet.t) n0 ig) eqn:H0.
-  - rewrite updateEntry_does_not_change_key_set.
-    rewrite updateEntry_does_not_change_key_set.
-    reflexivity.
-  - reflexivity.
-Qed.
-
-
-Lemma insEdges_does_not_add_nodes : forall (edges : list (Node * Node)) (ig : IG) (x : Node),
-  In x (labNodes (insEdges edges ig)) <-> In x (labNodes ig).
-Proof.
-  intros. simpl. induction edges.
-  - simpl. reflexivity.
-  - simpl. rewrite insEdge_does_not_add_node. rewrite IHedges. reflexivity.
-Qed. 
-
-
-Lemma insNode_any_ins_node : forall (node : Node) (ig : IG) (x : Node),
-  In x (labNodes (insNode node ig)) <-> In x (node :: labNodes ig).
-Proof.
-  intros. simpl. unfold insNode.
-  rewrite In_labNodes_is_InMap. rewrite WF.add_in_iff.
-  rewrite In_labNodes_is_InMap.
-  reflexivity.
-Qed.  
-
-
-Lemma insNodes_any_ins_all_nodes : forall (nodes : list Node) (ig : IG) (x : Node),
-  In x (labNodes (insNodes nodes ig)) <-> In x (nodes ++ labNodes ig).
-Proof.
-  intros. induction nodes.
-    - simpl. reflexivity.
-    - simpl. rewrite insNode_any_ins_node. simpl. rewrite IHnodes. reflexivity.
-Qed.
-
-Lemma insEdge_on_empty_is_empty : forall (edge : Node * Node),
-  insEdge edge empty = empty.
-(* This proof is very similar to "insEdge_does_not_add_node", but using it here it is more complicated than just doing it again  *)
-Proof.
-  intros. unfold insEdge. destruct edge.
-  destruct (NatMap.mem (elt:=NatSet.t * NatSet.t) n empty && NatMap.mem (elt:=NatSet.t * NatSet.t) n0 empty) eqn:cond.
-  - compute. reflexivity.
-  - reflexivity.
-Qed. 
-
-
-Lemma insEdges_on_empty_is_empty : forall (edges : list (Node * Node)),
-  insEdges edges empty = empty.
-(* This proof is very similar to "insEdges_does_not_add_nodes", but using it here it is more complicated than just doing it again  *)
-Proof.
-  intros. induction edges; simpl.
-  - reflexivity.
-  - rewrite IHedges. rewrite insEdge_on_empty_is_empty. reflexivity.
-Qed.
-
-
-
-(* "big" statement: *)
-Theorem mkGraph_any_ins_all_nodes : forall (nl : list Node) (el : list (Node * Node)) (x : Node),
-  In x (labNodes (mkGraph nl el)) <-> In x nl.
-Proof.
-  intros. unfold mkGraph. rewrite insEdges_does_not_add_nodes. rewrite insNodes_any_ins_all_nodes.
-  rewrite app_nil_r. reflexivity.
-Qed.
-
-
-Theorem empty_isEmpty : isEmpty empty = true.
-Proof.
-  compute. reflexivity.
-Qed.
-
-Theorem labNodes_empty_nil : labNodes empty = [].
-Proof.
-  compute. reflexivity.
-Qed.
-
-
-(* Protipp: firstorder and congruence seem pretty useful *)
-Lemma not_NatMap_Empty_is_empty_false : forall (A : Type) (m : NatMap.t A), not (NatMap.Empty m) <-> NatMap.is_empty m = false.
-Proof.
-  intros. unfold not. rewrite WF.is_empty_iff. destruct (NatMap.is_empty (elt:=A) m) eqn:cond.
-  - firstorder. congruence.
-  - firstorder. congruence.
-Qed.
-
-
-Theorem  non_empty_isEmpty_false : forall (nodes : list Node) (edges : list (Node * Node)),
-  length nodes <> 0 <-> isEmpty ((mkGraph nodes edges)) = false.
-Proof.
-  intros. unfold isEmpty. rewrite <- not_NatMap_Empty_is_empty_false. unfold not.
-  destruct nodes; simpl; unfold mkGraph.
-  - firstorder.
-    apply H.
-    apply WP.elements_Empty.
-
-    rewrite insEdges_on_empty_is_empty. compute. reflexivity.
-  - firstorder.
-    + apply WP.elements_Empty in H0.
-      assert (HH : not (exists e, InA (fun x el : Node * (NatSet.t * NatSet.t) => x = el) (n, e) [])). {
-        unfold not. intros. destruct H1. inversion H1.
-      }
-      rewrite <- In_conditions_same in HH.
-
-      unfold not in HH. apply HH.
-      
-      pose proof WF.elements_in_iff.
-      edestruct H1.
-      rewrite H0 in H2.
-      apply H2.
-      
-      apply In_labNodes_is_InMap.
-      apply mkGraph_any_ins_all_nodes. simpl. left. reflexivity.
-    + congruence.
-Qed.
-
-
-
-Theorem matsh_empty_is_nothing : forall (node : Node), matsh node empty = (None, empty).
-Proof.
-  intros. compute. reflexivity.
-Qed.
-
-
-Theorem spec4 : forall (node : Node) (nodes : list Node) (edges : list (Node * Node)), 
-  In node nodes -> exists froms tos, matsh node (mkGraph nodes edges) =
-  (Some (froms, tos), mkGraph (filter (fun n => negb (node =? n)) nodes) (filter (fun '(from, to) => negb ((from =? node) || (to =? node))) edges)).
-(* This is not even a complete specification and it looks like a hard one to prove... *)
-Proof.
-Admitted.
-
-
-Theorem spec5 : forall (node : Node) (nodes : list Node) (edges : list (Node * Node)), 
-  not (In node nodes) -> matsh node (mkGraph nodes edges) = (None, mkGraph nodes edges).
-Proof.
-Admitted.
