project/inductive/basic/inductive_graph_basic_theory.v
@@ -1,316 +1,231 @@
-Require Import String.
+Require Import Coq.micromega.Lia.
+Require Import Coq.Logic.FunctionalExtensionality.
+Require Import Coq.Logic.PropExtensionality.
+
 Require Import Coq.Arith.Arith.
-Open Scope string_scope.
 
 Require Import List.
+Require Import Coq.Structures.OrdersTac.
 Require Import Bool.
 Import ListNotations.
 
+Require Import FSets.
+Require Import FMaps.
+Require Import OrderedTypeEx.
+
 Require Import MyProject.project.inductive.basic.inductive_graph_basic.
-Require Import MyProject.project.relational_graph.
 
-Require Import Coq.Sets.Ensembles.
-
-
-(* Defining Conversion from basic Inductive Graph to Relational Graph *)
-
-(* This works better in proofs than the library Add for ensembles *)
-Definition _customEnsembleAdd {A : Type} (a : A) (en : Ensemble A) : Ensemble A :=
-  fun (x : A) => x = a \/ en x
-.
-
-Definition _listToEnsemble {A : Type} (az : list A) : Ensemble A :=
-  fold_right _customEnsembleAdd (Empty_set A) az
-.
+(* (attempt at) direct equational specifications of an IG_basic: *)
 
 
-(* Adds a node and its in- and out- going edges (= its IG context) to an RG.
-    Assumes that the neighboring nodes exist *)
-Definition _extendByContext (node : Node) (froms tos : NatSet.t) (rg : RG nat) : RG nat.
+(* Block to derive useful conversion theorem "In_labNodes_is_InMap" *)
+
+
+(* Helper lemma for converting an In (of a map) to an InA, which will eventually be turned to a NatMap.In (which has useful lemmas)  *)
+Lemma In_map_fst_InA : forall (A B: Type) (a : A) (l : list (A * B)),
+  In a (map fst l) <-> exists (a0 : B), InA (fun (x el : (A * B)) => x = el) (a, a0) l.
 Proof.
-    refine {|
-        RG_nodes := fun (n : nat) => NatSet.In n froms \/ NatSet.In n tos \/ (_customEnsembleAdd node rg.(RG_nodes))  n;
-        RG_edges := fun (n0 n1 : nat) =>
-                                (NatSet.In n0 froms /\ n1 = node)
-                                \/ (n0 = node /\ NatSet.In n1 tos)
-                                \/ rg.(RG_edges) n0 n1
-                                ;
-                     
-        RG_valid := _
-    |}.
-    RG_valid_prover_with rg.
-Defined.
+  intros. induction l; simpl.
+  - split; intros.
+    + destruct H.
+    + destruct H. inversion H.
+  - split; intros.
+    + destruct H.
+      -- exists (snd a0). left. destruct a0. destruct H. simpl. reflexivity.
+      -- edestruct IHl. apply H0 in H. destruct H. exists x. apply InA_cons. right. assumption.
+    + destruct H. inversion H.
+      -- left. destruct a0. destruct H1. simpl. reflexivity.
+      -- right. apply IHl. exists x. assumption.
+Qed.  
 
 
 
-
-Definition _accTo_RG (node : Node) (rgIg : RG nat * IG) : RG nat * IG :=
-    match rgIg with | (rg, ig) =>
-        match matsh node ig with
-        | (Some (froms, tos), rest) => (_extendByContext node froms tos rg, rest)
-        | (None, sameIg)            => (rg, sameIg)
-        end
-    end
-.
-
-Definition IG_basic_to_RG (ig : IG) : RG nat :=
-    match fold_right _accTo_RG (RG_empty, ig) (labNodes ig) with
-    | (rg, acc) => rg
-    end
-.
-
-
-(* Coercion IG_basic_to_RG : IG >-> RG. *)
-
-Definition IG_equiv (ig1 ig2 : IG) : Prop :=
-    RG_equiv (IG_basic_to_RG ig1) (IG_basic_to_RG ig2)
-.
-
-Notation "g1 I== g2" := (IG_equiv g1 g2) (at level 80).
-
-
-(* Section to make rewrite work with IG_equiv *)
-
-(* Source for rewrite: https://stackoverflow.com/questions/56099646/use-rewrite-tactic-with-my-own-operator-in-coq *)
-Require Import Setoid Morphisms.
-
-(* This proof is based on === being an equivalence relation *)
-Instance IG_Equivalence_eq : Equivalence IG_equiv.
+(* Conversion from key equality from map to my own (simply written in a slightly different manner) *)
+Lemma In_conditions_same : (NatMap.eq_key_elt (elt:=NatSet.t * NatSet.t)) = (fun x el : Node * (NatSet.t * NatSet.t) => x = el).
 Proof.
-    pose proof (@RG_Equivalence_eq nat). destruct H. split.
-    - unfold Reflexive. intros. unfold Reflexive in Equivalence_Reflexive. apply Equivalence_Reflexive.
-    - unfold Symmetric. intros. unfold Symmetric in Equivalence_Symmetric. apply Equivalence_Symmetric. apply H.
-    - unfold Transitive. intros. unfold Transitive in Equivalence_Transitive. apply (Equivalence_Transitive _ (IG_basic_to_RG y) _).
-        + apply H.
-        + apply H0.
-Qed. 
-
-
-Example basic_equivalence_test : (mkGraph [1; 2] []) I== (mkGraph [2; 1] []).
-Proof.
-    unfold IG_equiv. unfold RG_equiv. firstorder.
+  unfold NatMap.eq_key_elt. unfold NatMap.Raw.PX.eqke.
+  apply functional_extensionality.
+  intros.
+  apply functional_extensionality.
+  intros.
+  destruct x, x0.
+  simpl.
+  apply propositional_extensionality.
+  split; intros.
+  - destruct H. subst. reflexivity.
+  - inversion H. auto.
 Qed.
 
-Example basic_equivalence_test' : (mkGraph [1; 2; 3] [(1, 2); (2, 3)]) I== (mkGraph [2; 1; 3] [(2, 3); (1, 2)]).
+(* This is the most useful one for proving other statements.
+  Use it to convert from "use friendly" In- statements to "provable" NatMap.In- statements  *)
+Lemma In_labNodes_is_InMap : forall (x : Node) (ig : IG),
+  In x (labNodes ig) <-> NatMap.In x ig.
 Proof.
-    unfold IG_equiv. unfold RG_equiv. firstorder.
+  intros. unfold labNodes.
+  rewrite In_map_fst_InA.
+  pose proof (WF.elements_in_iff ig).
+  rewrite In_conditions_same in H.
+  specialize H with x.
+  symmetry.
+  assumption.
 Qed.
 
-
-
-(* Now start defining the basic IG functions in terms of an RG *)
-  (* {-# MINIMAL empty, isEmpty, match, mkGraph, labNodes #-} *)
-
-
-(* Start defining functionality: *)
-Definition RG_empty : RG nat :=
-    RG_empty.
-
-
-Definition RG_isEmpty (rg : RG nat) : Prop :=
-  RG_isEmpty rg.
-
-
-
-(* Helper for matsh *)
-Definition _eliminate (node : Node) (rg : RG nat) : RG nat.
-Proof.
-  refine {|
-      RG_nodes := Subtract nat (rg.(RG_nodes)) node;
-      RG_edges := fun (n0 n1 : nat) => n0 <> node /\ n1 <> node /\  rg.(RG_edges) n0 n1;
-      RG_valid := _
-  |}.
-  RG_valid_prover_with rg.
-  - unfold not. intros. inversion H2. congruence.
-  - unfold not. intros. inversion H2. congruence.
-Defined.
-
-Definition _getFromsAndTos (node : Node) (rg : RG nat) : Prop * (Ensemble nat * Ensemble nat) :=
-  (rg.(RG_nodes) node, ((fun (from : nat) => rg.(RG_edges) from node), (fun (to : nat) => rg.(RG_edges) node to)))
-.
-
-
-(* (Ensemble nat * Ensemble nat) is not a relation, it is two _independent_ sets of from- and to- neighbors *)
-Definition RG_matsh (node : Node) (rg : RG nat) : (Prop * (Ensemble nat * Ensemble nat)) * RG nat :=
-  (_getFromsAndTos node rg, _eliminate node rg)
-.
-
-
-
-Definition _add (node : Node) (fromsTos : (NatSet.t * NatSet.t)) (rg : RG nat) : RG nat :=
-  match fromsTos with | (froms, tos) =>
-    _extendByContext node froms tos rg
-  end
-.
-
-
-Definition _insNode (node : Node) (rg : RG nat) : RG nat :=
-  _add node (NatSet.empty, NatSet.empty) rg.
-  
-
-Definition _insNodes (nodes : list Node) (rg : RG nat) : RG nat :=
-  fold_right _insNode rg nodes.
-
-
-(* If one of the nodes of the edge does not exist, nothing happens *)
-Definition _insEdge (edge : (Node * Node)) (rg : RG nat) : RG nat.
-Proof.
-  destruct edge as [node0 node1].
-    refine {|
-      RG_nodes := rg.(RG_nodes);
-      RG_edges := fun (n0 n1 : nat) => (n0 = node0 /\ n1 = node1 /\ rg.(RG_nodes) node0 /\ rg.(RG_nodes) node1) \/  rg.(RG_edges) n0 n1;
-      RG_valid := _
-  |}.
-  RG_valid_prover_with rg.
-  - congruence.
-  - congruence.
-Defined.
-
-
-Definition _insEdges (edges : list (Node * Node)) (rg : RG nat) : RG nat :=
-  fold_right _insEdge rg edges.
-
-Definition RG_mkGraph (nodes : list Node) (edges : list (Node * Node)) : RG nat :=
-  _insEdges edges (_insNodes nodes RG_empty).
- 
-Definition RG_labNodes (rg : RG nat) : Ensemble Node :=
-  rg.(RG_nodes).
-
-
-(* Here come some proofs about equations: *)
 
 (* Here start "meaningful statements" *)
 
-(* 5 statements on inserting (helpers for mkGraph): update, insEdge, insEdges, insNode, insNodes *)
 
-Lemma RG_insEdge_does_not_add_node : forall (edge : (Node * Node)) (rg : RG nat),
-  RG_labNodes (_insEdge edge rg) = RG_labNodes rg.
+(* 5 statements on inserting (helpers for mkGraph): update, insEdge, insEdges, insNode, insNodes *)
+Lemma updateEntry_does_not_change_key_set : forall (node : Node) (f : NatSet.t * NatSet.t -> NatSet.t * NatSet.t) (ig : IG) (x : Node),
+  In x (labNodes (updateEntry node f ig)) <-> In x (labNodes ig).
 Proof.
-  intros. simpl. unfold RG_labNodes. unfold _insEdge. destruct edge. simpl. reflexivity.
+  intros. unfold updateEntry.
+  destruct (NatMap.find (elt:=NatSet.t * NatSet.t) node ig) eqn:isIn.
+  - rewrite In_labNodes_is_InMap. rewrite In_labNodes_is_InMap. rewrite WF.add_in_iff.
+    rewrite WF.in_find_iff. split.
+    + intros. destruct H.
+      -- rewrite <- H. rewrite isIn. unfold not. intros. discriminate H0.
+      -- assumption.
+    + intros. right. assumption.
+  - reflexivity.
 Qed.
 
 
-Lemma RG_insEdges_does_not_add_nodes : forall (edges : list (Node * Node)) (rg : RG nat),
-  RG_labNodes (_insEdges edges rg) = RG_labNodes rg.
+Lemma insEdge_does_not_add_node : forall (edge : (Node * Node)) (ig : IG) (x : Node),
+  In x (labNodes (insEdge edge ig)) <-> In x (labNodes ig).
 Proof.
-Admitted.
+  intros. unfold insEdge. destruct edge.
+  destruct (NatMap.mem (elt:=NatSet.t * NatSet.t) n ig && NatMap.mem (elt:=NatSet.t * NatSet.t) n0 ig) eqn:H0.
+  - rewrite updateEntry_does_not_change_key_set.
+    rewrite updateEntry_does_not_change_key_set.
+    reflexivity.
+  - reflexivity.
+Qed.
 
 
-Lemma RG_insNode_any_ins_node : forall (node : Node) (rg : RG nat),
-  RG_labNodes (_insNode node rg) = _customEnsembleAdd node (RG_labNodes rg).
+Lemma insEdges_does_not_add_nodes : forall (edges : list (Node * Node)) (ig : IG) (x : Node),
+  In x (labNodes (insEdges edges ig)) <-> In x (labNodes ig).
 Proof.
-Admitted.
+  intros. simpl. induction edges.
+  - simpl. reflexivity.
+  - simpl. rewrite insEdge_does_not_add_node. rewrite IHedges. reflexivity.
+Qed. 
 
 
-
-
-Lemma RG_insNodes_any_ins_all_nodes : forall (nodes : list Node) (rg : RG nat),
-  RG_labNodes (_insNodes nodes rg) = Union nat (_listToEnsemble nodes) (RG_labNodes rg).
+Lemma insNode_any_ins_node : forall (node : Node) (ig : IG) (x : Node),
+  In x (labNodes (insNode node ig)) <-> In x (node :: labNodes ig).
 Proof.
-Admitted.
+  intros. simpl. unfold insNode.
+  rewrite In_labNodes_is_InMap. rewrite WF.add_in_iff.
+  rewrite In_labNodes_is_InMap.
+  reflexivity.
+Qed.  
 
 
-
-Lemma RG_insEdge_on_empty_is_empty : forall (edge : Node * Node),
-  _insEdge edge RG_empty = RG_empty.
+Lemma insNodes_any_ins_all_nodes : forall (nodes : list Node) (ig : IG) (x : Node),
+  In x (labNodes (insNodes nodes ig)) <-> In x (nodes ++ labNodes ig).
 Proof.
-Admitted.
+  intros. induction nodes.
+    - simpl. reflexivity.
+    - simpl. rewrite insNode_any_ins_node. simpl. rewrite IHnodes. reflexivity.
+Qed.
+
+Lemma insEdge_on_empty_is_empty : forall (edge : Node * Node),
+  insEdge edge empty = empty.
+(* This proof is very similar to "insEdge_does_not_add_node", but using it here it is more complicated than just doing it again  *)
+Proof.
+  intros. unfold insEdge. destruct edge.
+  destruct (NatMap.mem (elt:=NatSet.t * NatSet.t) n empty && NatMap.mem (elt:=NatSet.t * NatSet.t) n0 empty) eqn:cond.
+  - compute. reflexivity.
+  - reflexivity.
+Qed. 
 
 
-Lemma RG_insEdges_on_empty_is_empty : forall (edges : list (Node * Node)),
-  _insEdges edges RG_empty = RG_empty.
+Lemma insEdges_on_empty_is_empty : forall (edges : list (Node * Node)),
+  insEdges edges empty = empty.
 (* This proof is very similar to "insEdges_does_not_add_nodes", but using it here it is more complicated than just doing it again  *)
 Proof.
-Admitted.
+  intros. induction edges; simpl.
+  - reflexivity.
+  - rewrite IHedges. rewrite insEdge_on_empty_is_empty. reflexivity.
+Qed.
 
 
 
 (* "big" statement: *)
-Theorem RG_mkGraph_any_ins_all_nodes : forall (nodes : list Node) (edges : list (Node * Node)),
-  RG_labNodes (RG_mkGraph nodes edges) = _listToEnsemble nodes.
+Theorem mkGraph_any_ins_all_nodes : forall (nl : list Node) (el : list (Node * Node)) (x : Node),
+  In x (labNodes (mkGraph nl el)) <-> In x nl.
 Proof.
-Admitted.
+  intros. unfold mkGraph. rewrite insEdges_does_not_add_nodes. rewrite insNodes_any_ins_all_nodes.
+  rewrite app_nil_r. reflexivity.
+Qed.
 
 
-Theorem RG_empty_isEmpty : RG_isEmpty RG_empty.
+Theorem empty_isEmpty : isEmpty empty = true.
 Proof.
   compute. reflexivity.
 Qed.
 
-Theorem RG_labNodes_empty_nil : RG_labNodes RG_empty = Empty_set nat.
+Theorem labNodes_empty_nil : labNodes empty = [].
 Proof.
-Admitted.
+  compute. reflexivity.
+Qed.
 
 
-
-Theorem RG_non_empty_isEmpty_false : forall (nodes : list Node) (edges : list (Node * Node)),
-  length nodes <> 0 <-> not (RG_isEmpty ((RG_mkGraph nodes edges))).
+(* Protipp: firstorder and congruence seem pretty useful *)
+Lemma not_NatMap_Empty_is_empty_false : forall (A : Type) (m : NatMap.t A), not (NatMap.Empty m) <-> NatMap.is_empty m = false.
 Proof.
-Admitted.
+  intros. unfold not. rewrite WF.is_empty_iff. destruct (NatMap.is_empty (elt:=A) m) eqn:cond.
+  - firstorder. congruence.
+  - firstorder. congruence.
+Qed.
 
 
-
-
-Theorem RG_matsh_empty_is_nothing : forall (node : Node),
-  RG_matsh node RG_empty = ((False, (Empty_set nat, Empty_set nat)), RG_empty).
+Theorem  non_empty_isEmpty_false : forall (nodes : list Node) (edges : list (Node * Node)),
+  length nodes <> 0 <-> isEmpty ((mkGraph nodes edges)) = false.
 Proof.
-Admitted.
+  intros. unfold isEmpty. rewrite <- not_NatMap_Empty_is_empty_false. unfold not.
+  destruct nodes; simpl; unfold mkGraph.
+  - firstorder.
+    apply H.
+    apply WP.elements_Empty.
+
+    rewrite insEdges_on_empty_is_empty. compute. reflexivity.
+  - firstorder.
+    + apply WP.elements_Empty in H0.
+      assert (HH : not (exists e, InA (fun x el : Node * (NatSet.t * NatSet.t) => x = el) (n, e) [])). {
+        unfold not. intros. destruct H1. inversion H1.
+      }
+      rewrite <- In_conditions_same in HH.
+
+      unfold not in HH. apply HH.
+      
+      pose proof WF.elements_in_iff.
+      edestruct H1.
+      rewrite H0 in H2.
+      apply H2.
+      
+      apply In_labNodes_is_InMap.
+      apply mkGraph_any_ins_all_nodes. simpl. left. reflexivity.
+    + congruence.
+Qed.
 
 
 
-Theorem RG_spec4 : forall (node : Node) (nodes : list Node) (edges : list (Node * Node)), 
-  List.In node nodes -> exists froms tos, RG_matsh node (RG_mkGraph nodes edges) =
-  ((True, (froms, tos)), RG_mkGraph (filter (fun n => negb (node =? n)) nodes) (filter (fun '(from, to) => negb ((from =? node) || (to =? node))) edges)).
+Theorem matsh_empty_is_nothing : forall (node : Node), matsh node empty = (None, empty).
+Proof.
+  intros. compute. reflexivity.
+Qed.
+
+
+Theorem spec4 : forall (node : Node) (nodes : list Node) (edges : list (Node * Node)), 
+  In node nodes -> exists froms tos, matsh node (mkGraph nodes edges) =
+  (Some (froms, tos), mkGraph (filter (fun n => negb (node =? n)) nodes) (filter (fun '(from, to) => negb ((from =? node) || (to =? node))) edges)).
 (* This is not even a complete specification and it looks like a hard one to prove... *)
 Proof.
 Admitted.
 
 
-Theorem RG_spec5 : forall (node : Node) (nodes : list Node) (edges : list (Node * Node)), 
-  not (List.In node nodes) -> RG_matsh node (RG_mkGraph nodes edges) = ((False, (Empty_set nat, Empty_set nat)), RG_mkGraph nodes edges).
-Proof.
-Admitted.
-
-
-(* Now go to proving that the implementations from IG basic relate to the RG ones *)
-(* Filling in all the admitteds, should suffice to show that IG_basic operations are equivalent to RG operations *)
-(* Hence, all theorems from one apply to the other *)
-(*   {-# MINIMAL empty, isEmpty, match, mkGraph, labNodes #-} *)
-Definition IG_basic_Propify_isEmpty (result : bool) : Prop.
-Proof.
-Admitted.
-
-Definition IG_basic_Propify_matsh (result : option (NatSet.t * NatSet.t) * IG) : (Prop * (Ensemble nat * Ensemble nat)) * RG nat.
-Proof.
-Admitted.
-
-Definition IG_basic_Propify_labNodes (result : list Node) : Ensemble Node.
-Proof.
-Admitted.
-
-
-Theorem IG_basic_empty_relate :
-  IG_basic_to_RG empty = RG_empty.
-Proof.
-Admitted.
-
-Theorem IG_basic_isEmpty_relate : forall (ig : IG),
-  IG_basic_Propify_isEmpty (isEmpty ig) = RG_isEmpty (IG_basic_to_RG ig).
-Proof.
-Admitted.
-
-
-Theorem IG_basic_matsh_relate : forall (node : Node) (ig : IG),
-  IG_basic_Propify_matsh (matsh node ig) = RG_matsh node (IG_basic_to_RG ig).
-Proof.
-Admitted.
-
-Theorem IG_basic_mkGraph_relate : forall (nodes : list Node) (edges : list (Node * Node)),
-  IG_basic_to_RG (mkGraph nodes edges) = RG_mkGraph nodes edges.
-Proof.
-Admitted.
-
-Theorem IG_basic_labNodes_relate : forall (ig : IG),
-  IG_basic_Propify_labNodes (labNodes ig) = RG_labNodes (IG_basic_to_RG ig).
+Theorem spec5 : forall (node : Node) (nodes : list Node) (edges : list (Node * Node)), 
+  not (In node nodes) -> matsh node (mkGraph nodes edges) = (None, mkGraph nodes edges).
 Proof.
 Admitted.
