project/inductive/inductive_graph_theory.v
@@ -1,62 +1,18 @@
 Require Import String.
 Require Import Coq.Arith.Arith.
-Open Scope string_scope.
 
 Require Import List.
 Require Import Bool.
 Import ListNotations.
 
-Require Import MyProject.project.inductive.inductive_graph.
 Require Import MyProject.project.relational_graph.
+Require Import MyProject.project.relational_graph_theory.
 
-(* Defining Conversion from Inductive Graph to Record Graph *)
+Require Import MyProject.project.inductive.inductive_graph.
+Require Import MyProject.project.inductive.inductive_graph_to_RG.
 
+Open Scope nat_scope.
 
-(* TODO: add some kind of well-formedness condition 
-( think of the BSt invariant, which insert does not break)
- What is the correctness invariant for an inductive graph? *)
-
- 
-
-Definition labEdges {A B : Type} (ig : IG A B) : list (LEdge B).
-Proof.
-Admitted. 
-
-(* TODO: finish this *)
-Definition IG_to_RG {A B : Type} (ig : IG A B) : RG A.
-Proof.
-    Print labNodes.
-    (* list of node labels *)
-    pose (nodes := map snd (labNodes ig)).
-    (* list of connections made by edges (drop labels)*)
-    pose (edges := map (fun (edge : LEdge B) => match edge with | (from, to, lab) => (lookup from ig, lookup to ig) end) (labEdges ig)).
-    
-    refine {|
-        RG_nodes := fun (a : A) =>
-                            fold_right (fun (v : A) (acc: Prop) => (a = v) \/ acc) False nodes;
-
-        RG_edges := fun (a1 a2 : A) =>
-                            fold_right (fun (e : (option A) * (option A)) (acc: Prop) => match e with
-                                | (Some from, Some to) => ((a1 = from) /\ (a2 = to)) \/ acc
-                                (* This case should never happen *)
-                                | _ => acc
-                                end) False edges;
-                     
-        RG_valid := _
-    |}.
-    RG_valid_prover.
-Admitted.
-
-
-
-
-
-Coercion IG_to_RG : IG >-> RG.
-
-Definition IG_equiv {A : Type} (ig1 ig2 : IG A unit) : Prop :=
-RG_equiv ig1 ig2.
-
-Notation "g1 I== g2" := (IG_equiv g1 g2) (at level 80).
 
 
 (* Section to make rewrite work with IG_equiv *)
@@ -76,15 +32,43 @@ Proof.
 Qed. 
 
 
-
-
-(* TODO: this is hard. Check if there are any theorems on the map interface, that I can use *)
 Example basic_equivalence_test : (mkGraph [(1, "1"); (2, "2")] []) I== (mkGraph [(2, "2"); (1, "1")] []).
 Proof.
-    unfold IG_equiv. unfold RG_equiv. simpl. split; split; intros.
-    - admit.
-    - admit.
-    - admit.
-    - admit.
+  unfold IG_equiv. unfold RG_equiv. simpl. split; split; intros.
+  - admit.
+  - admit.
+  - admit.
+  - admit.
+Admitted.
+
+
+
+
+(* (attempt at) direct equational specifications of an IG: *)
+
+
+Theorem spec1 : forall A B, isEmpty (@empty A B) = true.
+Proof.
+  intros. compute. reflexivity.
+Qed.
+
+Theorem spec2 : forall (A B : Type) (nl : list (LNode A)) (el : list (LEdge B)), labNodes (mkGraph nl el) = nl.
+Proof.
+  intros. compute.
+Admitted.
+
+Theorem spec3 : forall (A B : Type) (n : node), matsh n (@empty A B) = (None, empty).
+Proof.
+  intros. compute.
+Admitted.
+
+Theorem spec4 : forall (A B : Type) (n : LNode A) (nl : list (LNode A)) (el : list (LEdge B)), 
+  In n nl -> exists map1 map2, matsh (fst n) (mkGraph nl el) =
+  (Some ((map1), snd n, (map2)), mkGraph (filter (fun '(idx, lab) => negb (fst n =? idx)) nl) (filter (fun '(to, from, lab) => negb ((to =? fst n) || (from =? fst n))) el)).
+(* This is not even a complete specification and it looks like a nightmare to prove... *)
+Admitted.
+
+Theorem spec5 : forall (A B : Type) (n : LNode A) (nl : list (LNode A)) (el : list (LEdge B)), 
+  not (In n nl) -> matsh (fst n) (mkGraph nl el) = (None, mkGraph nl el).
 Admitted.
 
