project/algebraic/algebraic_graph_to_RG.v
@@ -1,0 +1,67 @@
+Require Import MyProject.project.algebraic.algebraic_graph.
+Require Import MyProject.project.relational_graph.
+(* Notice how this file does not need relational_graph_theory  *)
+(* Require Import MyProject.project.relational_graph_theory. *)
+
+
+(* Defining Conversion from Algebraic Graph to Record Graph *)
+Definition empty_RG {A : Type} : RG A.
+Proof.
+    exact RG_empty.
+Defined.
+
+
+Definition singleton_RG {A : Type} (a : A) : RG A.
+Proof.
+    refine {|
+        RG_nodes := fun (x : A) => a = x;
+        RG_edges := fun x y => False;
+        RG_valid := _
+    |}.
+    RG_valid_prover.
+Defined.
+
+
+Definition overlay_RG {A : Type} (rg1 rg2 : RG A) : RG A.
+Proof.
+    refine {|
+        RG_nodes := fun A => (rg1.(RG_nodes) A) \/ (rg2.(RG_nodes) A);
+        RG_edges := fun A B => (rg1.(RG_edges) A B) \/ (rg2.(RG_edges) A B);
+        RG_valid := _
+    |}.
+    RG_valid_prover_withs rg1 rg2.
+Defined.
+
+
+
+Definition connect_RG {A : Type} (rg1 rg2 : RG A) : RG A.
+Proof.
+    let overlay := constr:(overlay_RG rg1 rg2) in
+    refine {|
+        RG_nodes := overlay.(RG_nodes);
+        RG_edges := fun A B => overlay.(RG_edges) A B \/ (rg1.(RG_nodes) A /\ rg2.(RG_nodes) B);
+        RG_valid := _
+    |}.
+    RG_valid_prover_withs rg1 rg2.
+Defined.
+
+
+
+
+Fixpoint AG_to_RG {A : Type} (ag : AG A) : RG A :=
+    match ag with
+    | Empty => empty_RG
+    | Vertex x => singleton_RG x
+    | Overlay ag1 ag2 => overlay_RG (AG_to_RG ag1) (AG_to_RG ag2)
+    | Connect ag1 ag2 => connect_RG (AG_to_RG ag1) (AG_to_RG ag2)
+    end
+.
+
+(* TODO: this coercion may or may not be good to have *)
+Coercion AG_to_RG : AG >-> RG.
+
+
+Definition AG_equiv {A : Type} (ag1 ag2 : AG A) : Prop :=
+    RG_equiv ag1 ag2.
+
+Notation "g1 A== g2" := (AG_equiv g1 g2) (at level 80).
