project/inductive/inductive_graph_to_RG.v
@@ -1,0 +1,59 @@
+Require Import String.
+Require Import Coq.Arith.Arith.
+Open Scope string_scope.
+
+Require Import List.
+Require Import Bool.
+Import ListNotations.
+
+Require Import MyProject.project.inductive.inductive_graph.
+Require Import MyProject.project.relational_graph.
+Require Import MyProject.project.relational_graph_theory.
+
+
+(* Defining Conversion from Inductive Graph to Record Graph, this is a work in progress *)
+
+
+(* TODO: add some kind of well-formedness condition 
+( think of the BSt invariant, which insert does not break)
+ What is the correctness invariant for an inductive graph? *)
+
+ 
+
+Definition labEdges {A B : Type} (ig : IG A B) : list (LEdge B).
+Proof.
+Admitted. 
+
+(* TODO: finish this *)
+Definition IG_to_RG {A B : Type} (ig : IG A B) : RG A.
+Proof.
+    Print labNodes.
+    (* list of node labels *)
+    pose (nodes := map snd (labNodes ig)).
+    (* list of connections made by edges (drop labels)*)
+    pose (edges := map (fun (edge : LEdge B) => match edge with | (from, to, lab) => (lookup from ig, lookup to ig) end) (labEdges ig)).
+    
+    refine {|
+        RG_nodes := fun (a : A) =>
+                            fold_right (fun (v : A) (acc: Prop) => (a = v) \/ acc) False nodes;
+
+        RG_edges := fun (a1 a2 : A) =>
+                            fold_right (fun (e : (option A) * (option A)) (acc: Prop) => match e with
+                                | (Some from, Some to) => ((a1 = from) /\ (a2 = to)) \/ acc
+                                (* This case should never happen *)
+                                | _ => acc
+                                end) False edges;
+                     
+        RG_valid := _
+    |}.
+    RG_valid_prover.
+Admitted.
+
+
+Coercion IG_to_RG : IG >-> RG.
+
+
+Definition IG_equiv {A : Type} (ig1 ig2 : IG A unit) : Prop :=
+    RG_equiv ig1 ig2.
+
+Notation "g1 I== g2" := (IG_equiv g1 g2) (at level 80).
