project/relational_graph.v
@@ -2,8 +2,7 @@ Require Import Coq.Relations.Relation_Definitions.
 Require Import Coq.Relations.Relation_Operators.
 Require Import Coq.Sets.Ensembles.
 
-
-(* Defining a Relational Graph *)
+(* Defining a Relational Graph and its (possible) operations *)
 
 
 Definition _valid_cond {A : Type} (nodes : Ensemble A) (rel : relation A) : Type :=
@@ -34,46 +33,9 @@ Definition RG_equiv {A : Type} (rg1 rg2 : RG A) : Prop :=
 Notation "g1 === g2" := (RG_equiv g1 g2) (at level 100, right associativity).
 
 
-(* "RG_equiv" is an equivalence relation: *)
-(* Reflexive *)
-Theorem RG_equiv_Reflexive {A : Type}: forall (rg : RG A), RG_equiv rg rg.
-Proof.
-    firstorder.
-Qed.
-    
-
-(* Symmetric *)
-Theorem RG_equiv_Symmetric {A : Type}: forall (rg1 rg2 : RG A), RG_equiv rg1 rg2 <-> RG_equiv rg2 rg1.
-Proof.
-    firstorder.
-Qed. 
-
-(* Transitive *)
-Theorem RG_equiv_Transitive {A : Type}: forall (rg1 rg2 rg3 : RG A), RG_equiv rg1 rg2 -> RG_equiv rg2 rg3 -> RG_equiv rg1 rg3.
-Proof.
-    firstorder.
-    - apply H1. apply H2. apply H3.
-    - apply H2. apply H1. apply H3.
-Qed.
-
-(* Section to make rewrite work with equiv_RG *)
-
-(* Source for rewrite: https://stackoverflow.com/questions/56099646/use-rewrite-tactic-with-my-own-operator-in-coq *)
-Require Import Setoid Morphisms.
-Instance RG_Equivalence_eq {A : Type} : Equivalence (@RG_equiv A).
-Proof.
-    unfold RG_equiv. split.
-    - unfold Reflexive. intros. pose proof (@RG_equiv_Reflexive A). apply H.
-    - unfold Symmetric. intros. pose proof (@RG_equiv_Symmetric A). apply H0. apply H.
-    - unfold Transitive. intros. pose proof (@RG_equiv_Transitive A). apply (H1 x y).
-        + apply H.
-        + apply H0.
-Qed.
-
-(* Defining Operations on RGs: *)
 
 
-
+(* Defining Basic Operations on RGs: *)
 
 Definition RG_empty {A : Type} : RG A.
 Proof.
@@ -123,7 +85,6 @@ Proof.
 Defined.
 
 
-
 (* Does not remove associated nodes *)
 Definition RG_removeEdge {A : Type} (from to : A) (rg : RG A) : RG A.
 Proof.
@@ -153,4 +114,6 @@ Definition RG_existsPath {A : Type} (node1 node2 : A) (rg : RG A) : Prop :=
     clos_trans A rg.(RG_edges) node1 node2.
 
 (* Start implementing search *)
+
+
 
