project/relational_graph_theory.v
@@ -1,0 +1,43 @@
+Require Import Coq.Relations.Relation_Definitions.
+Require Import Coq.Relations.Relation_Operators.
+Require Import Coq.Sets.Ensembles.
+
+Require Import MyProject.project.relational_graph.
+
+(* Stated and proves Lemmas and Theorems about RGs *)
+
+(* "RG_equiv" is an equivalence relation: *)
+(* Reflexive *)
+Theorem RG_equiv_Reflexive {A : Type}: forall (rg : RG A), RG_equiv rg rg.
+Proof.
+    firstorder.
+Qed.
+    
+
+(* Symmetric *)
+Theorem RG_equiv_Symmetric {A : Type}: forall (rg1 rg2 : RG A), RG_equiv rg1 rg2 <-> RG_equiv rg2 rg1.
+Proof.
+    firstorder.
+Qed. 
+
+(* Transitive *)
+Theorem RG_equiv_Transitive {A : Type}: forall (rg1 rg2 rg3 : RG A), RG_equiv rg1 rg2 -> RG_equiv rg2 rg3 -> RG_equiv rg1 rg3.
+Proof.
+    firstorder.
+    - apply H1. apply H2. apply H3.
+    - apply H2. apply H1. apply H3.
+Qed.
+
+(* Section to make rewrite work with equiv_RG *)
+
+(* Source for rewrite: https://stackoverflow.com/questions/56099646/use-rewrite-tactic-with-my-own-operator-in-coq *)
+Require Import Setoid Morphisms.
+Instance RG_Equivalence_eq {A : Type} : Equivalence (@RG_equiv A).
+Proof.
+    unfold RG_equiv. split.
+    - unfold Reflexive. intros. pose proof (@RG_equiv_Reflexive A). apply H.
+    - unfold Symmetric. intros. pose proof (@RG_equiv_Symmetric A). apply H0. apply H.
+    - unfold Transitive. intros. pose proof (@RG_equiv_Transitive A). apply (H1 x y).
+        + apply H.
+        + apply H0.
+Qed.
