project/scrapped_examples/examples.v
@@ -1,12 +1,25 @@
 Require Import Coq.Relations.Relation_Definitions.
 Require Import Coq.Sets.Ensembles.
 Require Import Coq.Relations.Relation_Operators.
-
+Require Import List.
+Import ListNotations.
+Require Import String.
+Open Scope string_scope.
 
 Require Import MyProject.project.relational_graph.
 
+Require Import MyProject.project.algebraic.algebraic_graph.
+Require Import MyProject.project.algebraic.algebraic_graph_to_RG.
+Require Import MyProject.project.algebraic.algebraic_graph_theory.
+
+Require Import MyProject.project.inductive.inductive_graph.
+
+
+
 (* Mini examples, I had in other files but I moved here for cleanness *)
 
+
+(* RGs --------------------------------------------------------------------------- *)
 (* Definition Powerset : Type -> Type :=
     fun X => X -> Prop. *)
 
@@ -46,3 +59,44 @@ Proof.
     - apply t_step. auto.
     - apply t_step. auto.
 Qed.
+
+
+(* AGs --------------------------------------------------------------------------- *)
+
+Theorem AG_equiv_rewrite_test_basic : forall (ag1 ag2 ag3 : AG nat), AG_equiv ag1 ag2 -> AG_equiv ag2 ag3 -> AG_equiv ag1 ag3.
+Proof.
+    intros. rewrite H. rewrite H0. reflexivity.
+Qed.
+
+
+Theorem AG_equiv_rewrite_test_advanced : forall (ag1 ag2 ag3 : AG nat), AG_equiv ag1 ag2 -> AG_equiv (ag2 +++ Empty) ag3 -> AG_equiv (ag1 +++ Empty) ag3.
+Proof.
+    intros. rewrite H. rewrite H0. reflexivity.
+Qed.
+
+
+
+
+
+
+
+
+(* IGs --------------------------------------------------------------------------- *)
+
+
+Compute show_IG (mkGraph [(1, 1); (2, 2); (3, 3)] [(1, 2, 1); (2, 3, 2); (3, 1, 3)]).
+
+Definition my_basic_graph := mkGraph [(1, "a"); (2, "b"); (3, "c")] [(1, 2, "edge1"); (2, 3, "edge2"); (3, 1, "edge3")].
+
+(* Here come the tests for each defined function (that is in the graph class): *)
+
+Compute show_IG empty.
+
+Compute isEmpty empty.
+Compute isEmpty my_basic_graph.
+
+Compute show_Decomp (matsh 2 my_basic_graph).
+
+Compute show_IG (mkGraph [(1, "a"); (2, "b"); (3, "c")] [(1, 2, "edge1"); (2, 3, "edge2"); (3, 1, "edge3")]).
+
+Compute labNodes my_basic_graph.
