project/util/util.v
@@ -1,0 +1,45 @@
+Require Import Bool.
+Require Import Coq.Arith.Arith.
+Require Import List.
+
+
+Require Import Coq.Sets.Ensembles.
+
+
+(* Utility things, that don't really belong anywhere else *)
+
+(* This works better in proofs than the library Add for ensembles *)
+Definition _customEnsembleAdd {A : Type} (a : A) (en : Ensemble A) : Ensemble A :=
+  fun (x : A) => x = a \/ en x
+.
+
+Definition _listToEnsemble {A : Type} (az : list A) : Ensemble A :=
+  fold_right _customEnsembleAdd (Empty_set A) az
+.
+
+
+(* This is from software foundations. Eventually, I will move this somewhere else *)
+Lemma eqb_reflect : forall x y, reflect (x = y) (x =? y).
+Proof.
+  intros x y. apply iff_reflect. symmetry.
+  apply Nat.eqb_eq.
+Qed.
+Lemma ltb_reflect : forall x y, reflect (x < y) (x <? y).
+Proof.
+  intros x y. apply iff_reflect. symmetry.
+  apply Nat.ltb_lt.
+Qed.
+Lemma leb_reflect : forall x y, reflect (x <= y) (x <=? y).
+Proof.
+  intros x y. apply iff_reflect. symmetry.
+  apply Nat.leb_le.
+Qed.
+
+Hint Resolve ltb_reflect leb_reflect eqb_reflect : bdestruct.
+Ltac bdestruct X :=
+  let H := fresh in let e := fresh "e" in
+   evar (e: Prop);
+   assert (H: reflect e X); subst e;
+    [ auto with bdestruct
+    | destruct H as [H|H];
+       [ | try first [apply not_lt in H | apply not_le in H]]].
